{\descr{Знайти Інтеграл}}

$$
  \int (x+5)\ln{x}\d{x} =
  \Bigg|
    \begin{array}{r l r l   }
        u  & = \ln{x} & v & = \dfrac{x^2}{2}+5x \\
        u' & = \dfrac{1}{x} & v' & = x+5  \\
      \end{array}
  \Bigg|
$$


$$
  \int (x+5)\ln{x}\d{x}
= \ln{x} (\dfrac{x^2}{2}+5x) - \int (\dfrac{x^2}{2}+5x) \dfrac{1}{x} \d{x}
$$
$$
= \ln{x} (\dfrac{x^2}{2}+5x) - \int \dfrac{x^2+10x}{2x}\d{x}
= \ln{x} (\dfrac{x^2}{2}+5x) - \dfrac{1}{2}\int \dfrac{x(x+10)}{x}\d{x}
$$

$$
= \ln{x} (\dfrac{x^2}{2}+5x) - \dfrac{1}{2} ( \int x\d{x} + \int 10\d{x} )
= \ln{x} (\dfrac{x^2}{2}+5x) - \dfrac{1}{2} ( \dfrac{x^2}{2} + 10x) + C
$$

$$
= \ln{x} (\dfrac{x^2}{2}+5x) - ( \dfrac{x^2}{4} + 5x) + C
= 5x\ln{x} + \dfrac{x^2}{2}\ln{x} - \dfrac{x^2}{4} - 5x + C
= 5x(\ln{x}-1) + \dfrac{1}{2}(\ln{x}-\dfrac{1}{2}) + C
$$

$$\boxed{5x(\ln{x}-1) + \dfrac{1}{2}(\ln{x}-\dfrac{1}{2}) + C}$$
