{\descr{Знайти Інтеграл}}


$$
  \int \dfrac{x\d{x}}{\sqrt{x^2+3x-1}}
= \int \dfrac{x\d{x}}{\sqrt{(x+\dfrac{3}{2})^2-\dfrac{13}{4}}}
= \Bigg |
  \begin{array}{rrrl}
    t = & x + \dfrac{3}{2} & \d{x} =& (x)'\d{t}\\
    \\
    x = & t - \dfrac{3}{2} & \d{x} =& \d{t}\\
  \end{array}
\Bigg |
= \int \dfrac{t-\dfrac{3}{2}}{\sqrt{t^2-\dfrac{13}{4}}} \d{t}
$$

$$
\int \dfrac{t\d{t}}{\sqrt{t^2-\dfrac{13}{4}}}  - \int \dfrac{\dfrac{3}{2}\d{t}}{\sqrt{t^2-\dfrac{13}{4}}}
= \int \dfrac{t\d{t}}{\sqrt{t^2-\dfrac{13}{4}}}  - \dfrac{3}{2} \int \dfrac{\d{t}}{\sqrt{t^2-\dfrac{13}{4}}}
=
$$

Окремо проінтегруємо обидва інтеграли:

$$
1)  \int \dfrac{t\d{t}}{\sqrt{t^2-\dfrac{13}{4}}}
= \int (t^2-\dfrac{13}{4})^{-\dfrac{1}{2}} \cdot t\d{t}
= \dfrac{2}{2} \int (t^2-\dfrac{13}{4})^{-\dfrac{1}{2}} \cdot t\d{t}
= \dfrac{1}{2} \int (t^2-\dfrac{13}{4})^{-\dfrac{1}{2}} \cdot 2t\d{t}
$$

$$
= \dfrac{1}{2} \int (t^2-\dfrac{13}{4})^{-\dfrac{1}{2}} \cdot \d{(t^2-\dfrac{13}{4})}
= \dfrac{2 \sqrt{t^2-\dfrac{13}{4}}}{2} + C
= \sqrt{(x + \dfrac{3}{2})^2-\dfrac{13}{4}} + C
= \sqrt{x^2+3x-1} + C.
$$


$$
2)
  - \dfrac{3}{2} \int \dfrac{\d{t}}{\sqrt{t^2-\dfrac{13}{4}}} = - \dfrac{3}{2}  ln \Bigg|t + \sqrt{t^2-\dfrac{13}{4}}\Bigg| + C = - \dfrac{3}{2}  ln \Bigg|x + \dfrac{3}{2} + \sqrt{(x + \dfrac{3}{2})^2-\dfrac{13}{4}}\Bigg| + C
$$

Підставимо обидва розвязки назад в нашу формулу і отримаємо рішення:

$$
\sqrt{x^2+3x-1} - \dfrac{3 \ln{\bigg|x + \dfrac{3}{2} + \sqrt{x^2+3x-1}\bigg|} }{2} + C
$$
