{\descr{Знайти Інтеграл}}

$$
  \int \dfrac{(x^2+23)\d{x}}{(x+1)(x^2+6x+13)}
$$

Спершу, cпрощуємо многочлен:
$$
  \dfrac{(x^2+23)\d{x}}{(x+1)(x^2+6x+13)}
= \dfrac{A}{(x+1)} + \dfrac{Bx+C}{(x^2+6x+13)}
= \dfrac{A(x^2+6x+13) + (Bx+C)(x+1)}{(x+1)(x^2+6x+13)}
$$
$$
  (x^2+23) = A(x^2+6x+13) + (Bx+C)(x+1) = Ax^2+6Ax+13A+Bx^2+Bx+Cx+C
$$

$$
  \begin{array}{rcl}
    x^2 & 0  & A+B\\
    x^1 & 1  & 6A+B+C\\
    x^0 & 23 & 13A+C
    \end{array}
    \hspace{2pt}
    {\text{з чого виходить що}}
    \hspace{2pt}
    A=3, B=-2, C=-16
$$

$$
  \int \dfrac{3}{x+1}\d{x} + \int \dfrac{-1(2x+16)}{x^2+6x+13}
= 3\int \dfrac{1}{x+1}\d{x} - \int \dfrac{2x+16}{x^2+6x+13}\d{x}
$$

$$
= 3\int \dfrac{1}{x+1}\d{x} - \int \dfrac{2x+6}{x^2+6x+13}\d{x} - \int \dfrac{10}{x^2+6x+13}\d{x}
$$

$$
= 3 \ln{|x+1|} + C - \int \dfrac{\d{x^2+6x+13}}{x^2+6x+13} - 10\int \dfrac{1}{x^2+6x+13}\d{x}
$$

$$
= 3 \ln{|x+1|} - \ln{|x^2+6x+13|} + C + 10\int \dfrac{1}{(x+3)^2+4}\d{x}
\Bigg|
  \begin{array}{rlrl}
    t = & x+3   & \d{x} = & (x)'\d{t}\\
    x = & t - 3 & \d{x} = & \d{t} \\
    \end{array}
\Bigg| =
$$

$$
  = 3 \ln{|x+1|} - \ln{|x^2+6x+13|} + C - 10\int \dfrac{1}{t^2+4}\d{t}
$$

$$
= 3 \ln{|x+1|} - \ln{|x^2+6x+13|} + C - \dfrac{10}{4}\int \dfrac{1}{\dfrac{t^2}{4}+1}\d{t}
\Bigg|
  \begin{array}{rlrl}
    u = & \dfrac{t}{2}   & \d{t} = & (t)'\d{u}\\
    t = & 2u & \d{t} = & 2\d{u} \\
    \end{array}
\Bigg|
$$

$$
= 3 \ln{|x+1|} - \ln{|x^2+6x+13|} + C - \dfrac{10}{4}\int \dfrac{2}{u^2+1}\d{u} = 3 \ln{|x+1|} - \ln{|x^2+6x+13|} + C - 5\int \dfrac{1}{u^2+1}\d{u}
$$

$$
= 3 \ln{|x+1|} - \ln{|x^2+6x+13|} - 5 \arctg{u} + C
= 3 \ln{|x+1|} - \ln{|x^2+6x+13|} - 5 \arctg{\dfrac{t}{2}} + C
$$

$$
\boxed{ 3 \ln{|x+1|} - \ln{|x^2+6x+13|} - 5 \arctg{\dfrac{x+3}{2}} + C }
$$
