{\descr{Знайти Інтеграл}}

$$
  \int \dfrac{\d{x}}{\sqrt[3]{1+x^3}}
$$

$\lhd I = x^-1 \codt (x^3+1)^{-1/3}  $ то $m=0$, $n=3$, $p=-\dfrac{1}{3}$ з чого випливає щомає місце $\dfrac{0+1}{3}+(-\dfrac{1}{3}) = 0, 0 \in \mathbb{Z} $, а отже ми використаємо підстановку $a+bx^n = x^n \cdot t^s$ (спрощено $\dfrac{a}{x^n}+b =t^s$), де $s$ знаменник $s$ .

$$
  \int \dfrac{\d{x}}{\sqrt[3]{1+x^3}} =
  \Bigg|
  \begin{array}{rl rl}
    t^3 =&  \dfrac{1}{x^3}+1   & \d{x} = & (x)'\d{t} \\
    x^3 =&  \dfrac{1}{t^3 - 1} & \d{x} = & t^{-4} \cdot (t^{-3}-1)^{-1/3} \d{t}  \\
    \end{array}
  \Bigg| = \int (1+\dfrac{1}{t^3-1})^{-1/3} \cdot t^{-4} \cdot (t^{-3}-1)^{-1/3} \d{t}
$$

$$
= \int \dfrac{1}{\sqrt[3]{1+\dfrac{1}{t^3-1}}} \cdot \dfrac{1}{t^4} \cdot \dfrac{1}{\sqrt[3]{\dfrac{1}{t^3}-1}}  \d{t}
= \int \dfrac{1}{t^4} \cdot \dfrac{1}{\sqrt[3]{(1+\dfrac{1}{t^3-1}) (\dfrac{1}{t^3}-1)}} \d{t}
= \int \dfrac{1}{t^4} \cdot \dfrac{1}{\sqrt[3]{(\dfrac{(t^3-1)+1}{t^3-1}) (\dfrac{1-t^3}{t^3})}} \d{t}
$$

$$
= \int \dfrac{1}{t^4} \cdot \dfrac{1}{\sqrt[3]{(\dfrac{t^3}{t^3-1}) (\dfrac{1-t^3}{t^3})}} \d{t}
= \int \dfrac{1}{t^4} \cdot \dfrac{1}{\sqrt[3]{\dfrac{1-t^3}{t^3-1}}} \d{t}
= \int \dfrac{1}{t^4} \cdot \dfrac{1}{\sqrt[3]{\dfrac{-t^3+1}{t^3-1}}} \d{t}
= \int \dfrac{1}{t^4} \cdot \dfrac{1}{\sqrt[3]{\dfrac{-(t^3-1)}{t^3-1}}} \d{t}
$$

$$
= \int \dfrac{1}{t^4} \cdot \dfrac{1}{\sqrt[3]{-1}} \d{t}
= \int \dfrac{1}{t^4} \cdot - \dfrac{1}{1} \d{t}
= - \int \dfrac{1}{t^4} \d{t}
= - \dfrac{1}{3t^3} + C
= - \dfrac{1}{3(\dfrac{1}{x^3}+1)} + C
= - \dfrac{1}{\dfrac{3+3x^3}{x^3}} + C
$$

$$
\boxed{- \dfrac{x^3}{3+3x^3} + C}
$$
