{\descr{Знайти похідну функції:}}

$$
x\tg{y}-y{\tg{x}} = 2
$$

$$
x\tg{y}-y{\tg{x}} - 2 = 0
$$

$$
 0 = (x\tg{y})'-(y{\tg{x}})' - (2)' = ( (x)'\tg{y} + x(\tg{y})' ) - ((y)'\tg{x} + y(\tg{x})') = (x'\tg{y} + \dfrac{x}{\cos^2{y}}) - (y'\tg{x}+\dfrac{y}{\cos^2{x}})
$$

$$
y'\tg{x}+\dfrac{y}{\cos^2{x}} = x'\tg{y} + \dfrac{x}{\cos^2{y}}
$$

$$
y'\tg{x}
  = x'\tg{y} + \dfrac{x}{\cos^2{y}} - \dfrac{y}{\cos^2{x}}
$$

$$
  y' = \dfrac{\tg{y}}{\tg{x}}   + \dfrac{x}{\tg{x}\cos^2{y}}   - \dfrac{y}{\tg{x}\cos^2{x}}
$$
